Sources/WasmToBoogie/obj/Debug/net9.0/WasmToBoogie.AssemblyInfo.cs
@@ -13,7 +13,7 @@ using System.Reflection;
 [assembly: System.Reflection.AssemblyCompanyAttribute("WasmToBoogie")]
 [assembly: System.Reflection.AssemblyConfigurationAttribute("Debug")]
 [assembly: System.Reflection.AssemblyFileVersionAttribute("1.0.0.0")]
-[assembly: System.Reflection.AssemblyInformationalVersionAttribute("1.0.0+59678c49e0565ecac23307cda08d588cadf4b122")]
+[assembly: System.Reflection.AssemblyInformationalVersionAttribute("1.0.0+10dcd5eca633c21d2f62193e78711596d61c07f2")]
 [assembly: System.Reflection.AssemblyProductAttribute("WasmToBoogie")]
 [assembly: System.Reflection.AssemblyTitleAttribute("WasmToBoogie")]
 [assembly: System.Reflection.AssemblyVersionAttribute("1.0.0.0")]
