corral_out.bpl
@@ -16,6 +16,12 @@ function real_to_bool(r: real) : bool;
 
 axiom (forall r: real :: { real_to_bool(r): bool } real_to_bool(r): bool <==> (if r == 0e0 then false else true));
 
+axiom (forall b: bool :: { bool_to_real(b) } bool_to_real(b) == 0e0 || bool_to_real(b) == 1e0);
+
+axiom (forall b: bool :: { real_to_bool(bool_to_real(b)) } real_to_bool(bool_to_real(b)) <==> b);
+
+axiom (forall r: real :: { real_to_bool(r) } real_to_bool(r) <==> false <==> r == 0e0);
+
 procedure InitRuntime();
   modifies $sp, $tmp1, $tmp2, $tmp3;
   ensures $sp == 0;
@@ -117,23 +123,19 @@ procedure pop();
 
 
 
-const MAX_REQUESTS: real;
-
-axiom MAX_REQUESTS == 1e1;
-
-var active_requests: real;
+var temp: real;
 
 procedure initGlobals();
-  modifies active_requests;
-  ensures active_requests == 0e0;
+  modifies temp;
+  ensures temp == 98e0;
 
 
 
-implementation initGlobals()
+implementation {:ForceInline} initGlobals()
 {
 
   anon0:
-    active_requests := 0e0;
+    temp := 98e0;
     return;
 }
 
@@ -160,91 +162,39 @@ implementation {:ForceInline} popArgs1() returns (a1: real)
 
 
 
-procedure acquire_request();
-  requires 0e0 <= active_requests && active_requests <= MAX_REQUESTS;
-  modifies $stack, $sp, $tmp1, $tmp2, active_requests;
-  ensures 0e0 <= active_requests && active_requests <= MAX_REQUESTS;
+procedure heat_step();
+  requires 0e0 <= temp && temp <= 1e2;
+  modifies $stack, $sp, $tmp1, $tmp2, temp;
+  ensures 0e0 <= temp && temp <= 1e2;
 
 
 
-implementation {:ForceInline} acquire_request()
+implementation {:ForceInline} heat_step()
 {
   var loc1: real;
-  var loc2: real;
   var entry_sp: int;
 
   anon0:
     entry_sp := $sp;
     loc1 := 0e0;
-    loc2 := 0e0;
-    call {:si_unique_call 0} push(active_requests);
+    call {:si_unique_call 0} push(temp);
     call {:si_unique_call 1} loc1 := popArgs1();
     call {:si_unique_call 2} push(loc1);
-    call {:si_unique_call 3} push(MAX_REQUESTS);
+    call {:si_unique_call 3} push(1e2);
     call {:si_unique_call 4} popToTmp1();
     call {:si_unique_call 5} popToTmp2();
-    call {:si_unique_call 6} push(bool_to_real($tmp2 >= $tmp1));
+    call {:si_unique_call 6} push(bool_to_real($tmp2 <= $tmp1));
     call {:si_unique_call 7} popToTmp1();
-    goto anon4_Then, anon4_Else;
-
-  anon4_Then:
-    assume {:partition} real_to_bool($tmp1);
-    call {:si_unique_call 8} push(0e0);
-    call {:si_unique_call 9} loc2 := popArgs1();
-    goto anon3;
-
-  anon4_Else:
-    assume {:partition} !real_to_bool($tmp1);
-    call {:si_unique_call 10} push(loc1);
-    call {:si_unique_call 11} push(11e0);
-    call {:si_unique_call 12} popToTmp1();
-    call {:si_unique_call 13} popToTmp2();
-    call {:si_unique_call 14} push($tmp2 + $tmp1);
-    call {:si_unique_call 15} active_requests := popArgs1();
-    call {:si_unique_call 16} push(1e0);
-    call {:si_unique_call 17} loc2 := popArgs1();
-    goto anon3;
-
-  anon3:
-    call {:si_unique_call 18} push(loc2);
-    return;
-}
-
-
-
-procedure release_request();
-  requires 0e0 <= active_requests && active_requests <= MAX_REQUESTS;
-  modifies $stack, $sp, $tmp1, $tmp2, active_requests;
-  ensures 0e0 <= active_requests && active_requests <= MAX_REQUESTS;
-
-
-
-implementation {:ForceInline} release_request()
-{
-  var loc1: real;
-  var entry_sp: int;
-
-  anon0:
-    entry_sp := $sp;
-    loc1 := 0e0;
-    call {:si_unique_call 19} push(active_requests);
-    call {:si_unique_call 20} loc1 := popArgs1();
-    call {:si_unique_call 21} push(loc1);
-    call {:si_unique_call 22} push(0e0);
-    call {:si_unique_call 23} popToTmp1();
-    call {:si_unique_call 24} popToTmp2();
-    call {:si_unique_call 25} push(bool_to_real($tmp2 > $tmp1));
-    call {:si_unique_call 26} popToTmp1();
     goto anon2_Then, anon2_Else;
 
   anon2_Then:
     assume {:partition} real_to_bool($tmp1);
-    call {:si_unique_call 27} push(loc1);
-    call {:si_unique_call 28} push(11e0);
-    call {:si_unique_call 29} popToTmp1();
-    call {:si_unique_call 30} popToTmp2();
-    call {:si_unique_call 31} push($tmp2 - $tmp1);
-    call {:si_unique_call 32} active_requests := popArgs1();
+    call {:si_unique_call 8} push(loc1);
+    call {:si_unique_call 9} push(1e0);
+    call {:si_unique_call 10} popToTmp1();
+    call {:si_unique_call 11} popToTmp2();
+    call {:si_unique_call 12} push($tmp2 + $tmp1);
+    call {:si_unique_call 13} temp := popArgs1();
     return;
 
   anon2_Else:
@@ -254,30 +204,56 @@ implementation {:ForceInline} release_request()
 
 
 
-procedure popDiscard1();
-  requires $sp >= 1;
-  modifies $sp;
-  ensures $sp == old($sp) - 1;
-  ensures 0 <= $sp;
+procedure cool_step();
+  requires 0e0 <= temp && temp <= 1e2;
+  modifies $stack, $sp, $tmp1, $tmp2, temp;
+  ensures 0e0 <= temp && temp <= 1e2;
 
 
 
-implementation {:ForceInline} popDiscard1()
+implementation {:ForceInline} cool_step()
 {
+  var loc1: real;
+  var entry_sp: int;
 
   anon0:
-    $sp := $sp - 1;
+    entry_sp := $sp;
+    loc1 := 0e0;
+    call {:si_unique_call 14} push(temp);
+    call {:si_unique_call 15} loc1 := popArgs1();
+    call {:si_unique_call 16} push(loc1);
+    call {:si_unique_call 17} push(1e0);
+    call {:si_unique_call 18} popToTmp1();
+    call {:si_unique_call 19} popToTmp2();
+    call {:si_unique_call 20} push(bool_to_real($tmp2 >= $tmp1));
+    call {:si_unique_call 21} popToTmp1();
+    goto anon2_Then, anon2_Else;
+
+  anon2_Then:
+    assume {:partition} real_to_bool($tmp1);
+    call {:si_unique_call 22} push(loc1);
+    call {:si_unique_call 23} push(1e0);
+    call {:si_unique_call 24} popToTmp1();
+    call {:si_unique_call 25} popToTmp2();
+    call {:si_unique_call 26} push($tmp2 - $tmp1);
+    call {:si_unique_call 27} temp := popArgs1();
+    return;
+
+  anon2_Else:
+    assume {:partition} !real_to_bool($tmp1);
     return;
 }
 
 
 
-procedure CorralChoice_request_spec();
-  modifies $stack, $sp, $tmp1, $tmp2, active_requests;
+procedure CorralChoice_sanity_check2_violeted();
+  requires 0e0 <= temp && temp <= 1e2;
+  modifies $stack, $sp, $tmp1, $tmp2, temp;
+  ensures 0e0 <= temp && temp <= 1e2;
 
 
 
-implementation {:ForceInline} CorralChoice_request_spec()
+implementation {:ForceInline} CorralChoice_sanity_check2_violeted()
 {
   var c: int;
 
@@ -288,8 +264,8 @@ implementation {:ForceInline} CorralChoice_request_spec()
 
   anon3_Then:
     assume {:partition} c == 0;
-    call {:si_unique_call 33} acquire_request();
-    call {:si_unique_call 34} popDiscard1();
+    call {:si_unique_call 28} heat_step();
+    assert 0e0 <= temp && temp <= 1e2;
     return;
 
   anon3_Else:
@@ -298,7 +274,8 @@ implementation {:ForceInline} CorralChoice_request_spec()
 
   anon4_Then:
     assume {:partition} c == 1;
-    call {:si_unique_call 35} release_request();
+    call {:si_unique_call 29} cool_step();
+    assert 0e0 <= temp && temp <= 1e2;
     return;
 
   anon4_Else:
@@ -308,24 +285,39 @@ implementation {:ForceInline} CorralChoice_request_spec()
 
 
 
-procedure BoogieEntry_request_spec();
-  modifies $sp, $tmp1, $tmp2, $tmp3, active_requests, $stack;
+procedure BoogieEntry_sanity_check2_violeted();
+  requires 0e0 <= temp && temp <= 1e2;
+  modifies $tmp1, $tmp2, $tmp3, $sp, $stack, temp;
+  ensures 0e0 <= temp && temp <= 1e2;
 
 
 
-implementation BoogieEntry_request_spec()
+procedure CorralEntry_sanity_check2_violeted();
+  requires 0e0 <= temp && temp <= 1e2;
+  modifies $sp, $tmp1, $tmp2, $tmp3, temp, $stack;
+  ensures 0e0 <= temp && temp <= 1e2;
+
+
+
+implementation CorralEntry_sanity_check2_violeted()
 {
 
   anon0:
-    call {:si_unique_call 36} InitRuntime();
-    call {:si_unique_call 37} initGlobals();
-    call {:si_unique_call 38} CorralChoice_request_spec();
+    call {:si_unique_call 30} InitRuntime();
+    call {:si_unique_call 31} initGlobals();
+    goto anon2_LoopHead;
+
+  anon2_LoopHead:
+    goto anon2_LoopDone, anon2_LoopBody;
+
+  anon2_LoopBody:
+    assume {:partition} true;
+    call {:si_unique_call 32} CorralChoice_sanity_check2_violeted();
+    goto anon2_LoopHead;
+
+  anon2_LoopDone:
+    assume {:partition} !true;
     return;
 }
-
-
-
-procedure CorralEntry_request_spec();
-  modifies $tmp1, $tmp2, $tmp3, $sp, $stack, active_requests;
 
 
